WIP; proving elimstack

helping/elim_stack/StackA.v
@@ -1,57 +1,29 @@
 Require Import CRIS.
 Require Import MemHeader MemA.
-Require Import SchHeader.
-From CRIS.helping Require Import Header.
+Require Import SchHeader SchA.
+From CRIS.helping Require Import Header HelpingTactics.
 Require Import StackHeader.
 
-Class stackG `{!crisG Γ Σ α β τ _S _I} := StackG {
+Class stackG (jobID retID : Type) `{!crisG Γ Σ α β τ _S _I} := StackG {
   stack_tokG :: inG (exclR unitO) Γ;
   stack_stateG :: inG (authR (optionUR $ exclR (listO (leibnizO val)))) Γ;
+  stack_helpingG :: inG (helpingR jobID retID) Γ;
 }.
-Definition stackΓ : HRA := #[exclR unitO; authR (optionUR $ exclR (listO (leibnizO val)))].
-Global Instance subG_stackG `{!crisG Γ Σ α β τ _S _I} : subG stackΓ Γ → stackG.
+Definition stackΓ (jobID retID : Type) : HRA :=
+  #[exclR unitO; authR (optionUR $ exclR (listO (leibnizO val))); helpingR jobID retID].
+Global Instance subG_stackG (jobID retID : Type) `{!crisG Γ Σ α β τ _S _I} :
+  subG (stackΓ jobID retID) Γ → (stackG jobID retID).
 Proof. solve_inG. Defined.
 Hint Unfold subG_stackG stack_tokG stack_stateG : GRA_index.
 
-Class SLRed `{Σ : GRA, @GATIntp.t (domain Σ) α} {n} (f : GTerm.t n) (P : iProp Σ) := {
-  SLRed_eq : ⟦f⟧ ⊣⊢ P
-}.
-Lemma SLRed_red `{S : SLRed n f P} : ⟦f⟧ ⊣⊢ P.
-Proof. destruct S; ss. Qed.
-
-Section instances.
-  Context `{!subG (Γ : HRA) Σ, !SL.G Γ Σ α β τ}.
-
-  Global Instance SLRed_own `{!inG M Γ, n : nat} (m : M) γ :
-    SLRed (n:=n) (<own> γ m)%SAT (own γ m).
-  Proof. econs; SL_red; eauto. Qed.
-
-  Global Instance SLRed_pure {n} (P : Prop) :
-    SLRed (⌜P⌝ : GTerm.t n)%SAT (⌜P⌝)%I.
-  Proof. econs; SL_red; eauto. Qed.
-
-  Global Instance SLRed_ex {A n} `{!STτ.t τ}
-      (f : A → GTerm.t n) (g : A → iProp Σ) `{∀ a, SLRed (f a) (g a)} :
-    SLRed (∃ a : τ{A}, f a)%SAT (∃ a, g a)%I.
-  Proof.
-    econs; SL_red; iSplit; iIntros "[%b H]"; iExists b; try rewrite SLRed_red //.
-  Qed.
-
-  Global Instance SLRed_and {n} (f g : GTerm.t n) P Q `{!SLRed f P, !SLRed g Q} :
-    SLRed (f ∧ g)%SAT (P ∧ Q).
-  Proof. econs; rewrite SLRed.and ?SLRed_red //. Qed.
-
-  Global Instance SLRed_or {n} (f g : GTerm.t n) P Q `{!SLRed f P, !SLRed g Q} :
-    SLRed (f ∨ g)%SAT (P ∨ Q).
-  Proof. econs; rewrite SLRed.or ?SLRed_red //. Qed.
-
-  Global Instance SLRed_sep {n} (f g : GTerm.t n) P Q `{!SLRed f P, !SLRed g Q} :
-    SLRed (f ∗ g)%SAT (P ∗ Q).
-  Proof. econs; rewrite SLRed.sepconj ?SLRed_red //. Qed.
-End instances.
+Global Instance SLRed_self `{!subG (Γ : HRA) Σ, !SL.G Γ Σ α β τ} {n} (f : GTerm.t n) :
+  SLRed f (⟦f, n⟧)%I | 6.
+Proof. econs; SL_red; eauto. Qed.
 
 Section definitions.
-  Context `{!crisG Γ Σ α β τ _S _I, !concG, !memG, !stackG} (N : namespace).
+  Definition jobID : Type := nat * nat * (val * val * gname).
+  Definition retID : Type := val.
+  Context `{!crisG Γ Σ α β τ _S _I, !concG, !memG, !stackG jobID retID, !newschG} (N : namespace).
 
   Let offerN := N .@ "offer".
   Let stackN := N .@ "stack".
@@ -65,12 +37,6 @@ Section definitions.
     iIntros "Hl1 Hl2".
     iCombine "Hl1 Hl2" gives %[]%auth_frag_op_valid_1.
   Qed.
-
-  (* Definition stack_elem_to_val (stack_rep : option val) : val :=
-    match stack_rep with
-    | None => Vint 0
-    | Some l => l
-    end. *)
 
   Fixpoint syn_list_inv (l : list val) (rep : val) (n : nat) : GTerm.t n :=
     match l with
@@ -122,83 +88,115 @@ Section definitions.
   Unshelve. all: try exact Vundef; try exact 1%Qp.
   Qed.
 
-  Definition syn_is_offer (γs : gname) (offer_rep : option val) (n : nat) : GTerm.t n :=
+  Definition syn_offer_inv n γo (offer : mblock * ptrofs) (jid : jobID) : GTerm.t n :=
+    (∃ (offerst : τ{val}) (rid : τ{nat}),
+      offer ↦ jid.2.1.2 ∗
+      (offer.1, offer.2 + 1)%Z ↦ offerst ∗
+      match offerst with
+      | Vint 0 => syn_helping_token n rid jid
+      | Vint 1 => syn_helping_done n rid Vundef
+      | _ => <own> γo (Excl ())
+      end)%SAT.
+
+  Definition offer_inv γo (offer : mblock * ptrofs) (jid : jobID) : iProp Σ :=
+    (∃ (offerst : val) (rid : nat),
+      offer ↦ jid.2.1.2 ∗
+      (offer.1, offer.2 + 1)%Z ↦ offerst ∗
+      match offerst with
+      | Vint 0 => helping_token rid jid
+      | Vint 1 => helping_done rid Vundef
+      | _ => own γo (Excl ())
+      end)%I.
+  Global Instance SLRed_offer_inv n γo offer jid :
+    SLRed (syn_offer_inv n γo offer jid) (offer_inv γo offer jid).
+  Proof.
+    econs; rewrite /syn_offer_inv /offer_inv ?SLRed_red; do 3 f_equiv; ii.
+    des_ifs; rewrite ?SLRed_red //.
+  Qed.
+  Definition syn_is_offer (γs : gname) (offer_rep : val) (n : nat) : GTerm.t n :=
     match offer_rep with
-    | None => ⊤
-    | Some l => ⊤
-      (* ∃ Q γo, inv offerN (offer_inv st_loc γo (stack_push_au γs v Q) Q) *)
+    | Vptr (offerb, offerofs) => 
+      ∃ (γo : τ{gname}) (jid : τ{jobID}),
+        syn_inv n offerN (syn_offer_inv n γo (offerb, offerofs) jid)
+    | _ => ⊤
     end%SAT.
 
-  Definition is_offer (γs : gname) (offer_rep : option val) (n : nat) : iProp Σ :=
-    match offer_rep with
-    | None => True
-    | Some l => True
-      (* ∃ Q γo, inv offerN (offer_inv st_loc γo (stack_push_au γs v Q) Q) *)
-    end%I.
-
-  Global Instance is_offer_SLRed γs offer_rep n :
-    SLRed (syn_is_offer γs offer_rep n) (is_offer γs offer_rep n).
-  Proof.
-    rewrite /syn_is_offer; destruct offer_rep; ss; econs; SL_red; eauto.
-  Qed.
-
-  Local Instance is_offer_persistent γs offer_rep n : Persistent (⟦syn_is_offer γs offer_rep n⟧).
-  Proof. rewrite SLRed_red. destruct offer_rep as [?|]; SL_red; apply _. Qed.
-
-  Definition offer_to_val (offer_rep : option val) : val :=
-    match offer_rep with
-    | None => Vint 0
-    | Some l => l
-    end.
-
   Definition syn_stack_inv (γs : gname) (stackb : mblock) (stackofs : ptrofs) (n : nat) : GTerm.t n :=
-    (∃ (stack_rep : τ{val}) (offer_rep : τ{option val}) (l : τ{list val}), <own> γs (● Excl' l) ∗
+    (∃ (stack_rep : τ{val}) (offer_rep : τ{val}) (l : τ{list val}), <own> γs (● Excl' l) ∗
        (stackb, stackofs) ↦ stack_rep ∗ syn_list_inv l stack_rep n ∗
-       (stackb, stackofs + 1)%Z ↦ offer_to_val offer_rep ∗ syn_is_offer γs offer_rep n)%SAT.
-
-  Definition stack_inv (γs : gname) (stackb : mblock) (stackofs : ptrofs) (n : nat) : iProp Σ :=
-    (∃ (stack_rep : val) (offer_rep : option val) (l : list val), own γs (● Excl' l) ∗
-      (stackb, stackofs) ↦ stack_rep ∗ list_inv l stack_rep n ∗
-      (stackb, stackofs + 1)%Z ↦ offer_to_val offer_rep ∗ is_offer γs offer_rep n)%I.
-
-  Global Instance stack_inv_SLRed γs stackb stackofs n :
-    SLRed (syn_stack_inv γs stackb stackofs n) (stack_inv γs stackb stackofs n).
-  Proof. rewrite /syn_stack_inv /stack_inv; econs; rewrite SLRed_red //. Qed.
+       (stackb, stackofs + 1)%Z ↦ offer_rep ∗ syn_is_offer γs offer_rep n)%SAT.
 
   Definition is_stack (γs : gname) (s : val) (n : nat) : iProp Σ :=
     (∃ (stackb : mblock) (stackofs : ptrofs),
       ⌜s = Vptr (stackb, stackofs)⌝ ∗ inv n stackN (syn_stack_inv γs stackb stackofs n))%I.
 
   Definition new_stack_spec : fspec :=
-    fspec_winv (↑N)
+    fspec_sch (↑N)
       (fspec_simple (λ _ : (),
         ((λ arg, ∃ (v : list val), ⌜arg = v↑⌝),
          (λ ret, ∃ v γs, ⌜ret = v↑⌝ ∗ is_stack γs v 0 ∗ stack_content γs []))%I)).
 
   Definition push_spec : fspec :=
-    fspec_winv (↑N)
-      (fspec_simple (λ '((s, v, l, γs) : val * val * list (leibnizO val) * gname),
-        ((λ arg, ⌜arg = [s; v]↑⌝ ∗ is_stack γs s 0 ∗ stack_content γs l),
-         (λ ret, ⌜ret = Vundef↑⌝ ∗ stack_content γs (v :: l)))%I)).
+    fspec_sch (↑N)
+      (fspec_simple (λ '((s, v, γs) : val * val * gname),
+        ((λ arg, ⌜arg = [s; v]↑⌝ ∗ is_stack γs s 0),
+         (λ ret, ⌜ret = Vundef↑⌝))))%I.
+
+  Definition pop_spec : fspec :=
+    fspec_sch (↑N)
+      (fspec_simple (λ '((s, γs) : val * gname),
+        ((λ arg, ⌜arg = [s]↑⌝ ∗ is_stack γs s 0),
+         (λ ret, True))))%I.
 End definitions.
 
+(* Temporary note : for this spec to make sense, pre/postconditions for atomic update should be
+   able to depend on the choice of the metavariable of the private pre/postconditions.
+   Thus, conventional Hoarefun is not usable for now. *)
 Module StackM. Section StackM.
-  Context `{!crisG Γ Σ α β τ _S _I, !concG, !memG, !stackG} (N : namespace).
+  Definition jobID : Type := nat * nat * (val * val * gname).
+  Definition retID : Type := val.
+
+  Context `{!crisG Γ Σ α β τ _S _I, !concG, !newschG, !memG, !stackG jobID retID}.
+  Context (mn : string) (N : namespace).
+
   (* Module definitions *)
   Definition scopes : list string := [].
 
-  (* Definition jobID : Type := val.
-  Definition jobCode : jobID → itree Helping.pureE unit :=
-    λ v, ret <- lat_img false (push_spec N) 𝒴 (Ret ()) v;; 𝒴;;; Ret ret. *)
+  Definition jobCode : jobID → itree Helping.pureE retID :=
+    λ '(_, _, (_, v, γs)),
+      l <- trigger (Take (list (leibnizO val)));;
+      trigger (Assume (stack_content γs l));;;
+      trigger (Guarantee (stack_content γs (v :: l)));;;
+      Ret Vundef.
+  Definition retCode : retID → Any.t := Any.upcast.
 
-  Definition new_stack : Any.t → itree crisE Any.t :=
-    λ arg, ret <- lat_img false (from_fspec (new_stack_spec N)) 𝒴 fbody_trivial arg;; 𝒴;;; Ret ret.
-  Definition push : Any.t → itree crisE Any.t :=
-    λ arg, ret <- lat_img true (from_fspec (push_spec N)) 𝒴 fbody_trivial arg;; 𝒴;;; Ret ret.
+  Definition new_stack : list val → itree crisE val :=
+    λ _, 𝒴;;; trigger (Choose val).
+
+  Definition push : list val → itree crisE val := λ arg,
+    x <- trigger (Take (meta (push_spec N)));;
+    trigger (Assume ((precond (push_spec N)) x arg↑ arg↑));;;
+    'vret : retID <- ccallU (Helping.run mn) x;;
+    trigger (Guarantee ((postcond (push_spec N)) x vret↑ vret↑));;;
+    Ret vret.
+
+  Definition pop : list val → itree crisE val := λ arg,
+    x <- trigger (Take (meta (pop_spec N)));;
+    trigger (Assume ((precond (pop_spec N)) x arg↑ arg↑));;;
+    𝒴;;;
+    '_ : () <- ccallU (Helping.help mn) ();;
+    l <- trigger (Take (list (leibnizO val)));;
+    trigger (Assume (stack_content x.2.2 l));;;
+    trigger (Guarantee (stack_content x.2.2 (tail l)));;;
+    let vret := match l with | v :: _ => v | _ => Vundef end in
+    𝒴;;;
+    trigger (Guarantee ((postcond (pop_spec N)) x vret↑ vret↑));;;
+    Ret vret.
 
   Definition fnsems : fnsems_type :=
-    [(Some StackHdr.new_stack, (true, wmask_all, scopes, (None, new_stack)));
-     (Some StackHdr.push,      (true, wmask_all, scopes, (None, push)))].
+    [(Some StackHdr.new_stack, (true, wmask_all, scopes, (Some (new_stack_spec N), cfunU new_stack)));
+     (Some StackHdr.push,      (true, wmask_all, scopes, (None, cfunU push)));
+     (Some StackHdr.pop,       (true, wmask_all, scopes, (None, cfunU pop)))].
 
   Program Definition Mod : SMod.t := {|
     SMod.scopes := scopes;
@@ -208,7 +206,7 @@ Module StackM. Section StackM.
   Solve All Obligations with prove_scope.
   Next Obligation. prove_nodup. Qed.
 
-  Definition t := Seal.sealing CRIS (SMod.to_mod sp_none Mod).
+  Definition t sp := Seal.sealing CRIS (SMod.to_mod sp Mod).
 End StackM. End StackM.
 
 (* Module StackA. Section StackA.
