helping/elim_stack/StackHeader.v
@@ -3,4 +3,5 @@ Require Import CRIS.
 Module StackHdr.
   Definition new_stack := "Stack.new_stack".
   Definition push := "Stack.push".
+  Definition pop := "Stack.pop".
 End StackHdr.
