helping/elim_stack/StackIA.v
@@ -1,95 +1,165 @@
 Require Import CRIS.
 Require Import ImpPrelude.
 Require Import MemTactics.
-Require Import SchHeader SchA SchTactics.
+Require Import SchHeader SchI SchA SchTactics.
 Require Import StackHeader StackA StackI.
+From CRIS.helping Require Import Header HelpingOn HelpingOnOffproof HelpingTactics.
+
+(* TEMP *)
+From iris.algebra Require Import gmap_view.
 
 Module StackIM. Section StackIM.
-  Context `{!crisG Γ Σ α β τ _S _I, !memG, Hsch : !newschG, !concG, !stackG} (N : namespace).
+  Context `{!crisG Γ Σ α β τ _S _I, !memG, Hsch : !newschG, !concG, !stackG StackM.jobID StackM.retID}.
+  Local Existing Instances stack_helpingG.
+
+  (* Helping module being parameterized by mn *)
+  Context (mn : string).
+
+  (* Stack module being masked for eliminating the helping module *)
+  Context (msk : string → bool) (N : namespace) (sp : sp_type).
+  Context (Hspsch : sp_incl (SchA.sp [] (↑N)) sp).
+  Context (Hsphelp : sp_incl ([(Some (Helping.run mn), None); (Some (Helping.help mn), None)]) sp).
+
+  (* Whitelist of functions callable in stack *)
+  Definition imp := omap id (Mod.exports SchI.t ++ Mod.exports MemA.t).
+  Context (Hmsk : wmask_sub (wmask_list imp) msk).
+
+  Lemma yield_msk : wmask_and msk wmask_all SchHdr.yield.
+  Proof.
+    revert Hmsk; rewrite /imp /wmask_and /wmask_list /wmask_sub; unfold_mod; ss.
+    intros Hmsk; simpl_bool; apply Hmsk; eauto.
+  Qed.
+  Lemma alloc_msk : wmask_and msk wmask_all MemHdr.alloc.
+  Proof.
+    revert Hmsk; rewrite /imp /wmask_and /wmask_list /wmask_sub; rewrite /MemA.t; unseal CRIS.
+    unfold_mod; ss.
+    intros Hmsk; simpl_bool; apply Hmsk; eauto.
+  Qed.
+  Lemma store_msk : wmask_and msk wmask_all MemHdr.store.
+  Proof.
+    revert Hmsk; rewrite /imp /wmask_and /wmask_list /wmask_sub; rewrite /MemA.t; unseal CRIS.
+    unfold_mod; ss.
+    intros Hmsk; simpl_bool; apply Hmsk; eauto.
+  Qed.
+  Lemma load_msk : wmask_and msk wmask_all MemHdr.load.
+  Proof.
+    revert Hmsk; rewrite /imp /wmask_and /wmask_list /wmask_sub; rewrite /MemA.t; unseal CRIS.
+    unfold_mod; ss.
+    intros Hmsk; simpl_bool; apply Hmsk; eauto.
+  Qed.
+  Lemma cas_msk : wmask_and msk wmask_all MemHdr.cas.
+  Proof.
+    revert Hmsk; rewrite /imp /wmask_and /wmask_list /wmask_sub; rewrite /MemA.t; unseal CRIS.
+    unfold_mod; ss.
+    intros Hmsk; simpl_bool; apply Hmsk; eauto.
+  Qed.
+  Lemma cmp_msk : wmask_and msk wmask_all MemHdr.cmp.
+  Proof.
+    revert Hmsk; rewrite /imp /wmask_and /wmask_list /wmask_sub; rewrite /MemA.t; unseal CRIS.
+    unfold_mod; ss.
+    intros Hmsk; simpl_bool; apply Hmsk; eauto.
+  Qed.
+  Hint Resolve yield_msk alloc_msk store_msk load_msk cas_msk cmp_msk : core.
 
   Definition init_cond : iProp Σ := emp%I.
 
   Local Definition MemA := MemA.t.
-  Local Definition StackM := StackM.t.
-  Local Definition StackI := StackI.t.
-  Local Definition IstFull := (IstProd (IstSB (Mod.scopes (StackM N)) IstTrue) IstEq).
-  Local Notation MA := (StackM N ★ MemA).
-  Local Notation MI := (StackI ★ MemA).
+  Local Definition SchI := CFilter.filter msk SchI.t.
+  Local Definition HelpingOn := HelpingOn.t mn StackM.jobCode StackM.retCode sp.
+  Local Definition StackM := (StackM.t mn N sp ★ MemA) ★ HelpingOn ★ SchI.
+  Local Definition StackI := CFilter.filter msk (StackI.t ★ MemA) ★ SchI.
+  Local Definition IstFull :=
+    (IstHelp StackM.jobID StackM.retID mn (IstProd ((IstSB (Mod.scopes StackM) IstTrue)) IstEq)).
 
   Let offerN := N .@ "offer".
   Let stackN := N .@ "stack".
 
-  Lemma new_stack_simF : ISim.sim_fun open MA MI init_cond IstFull (Some StackHdr.new_stack).
-  Proof using Hsch.
+  Lemma new_stack_simF :
+    ISim.sim_fun open StackM StackI init_cond IstFull (Some StackHdr.new_stack).
+  Proof using Hsch Hmsk.
     init_simF.
-    steps_l. unfold_lat_img_l.
+    steps_l. rename _q3 into stid, _q4 into mtid.
+    iDestruct "ASM" as "[TID [[%v ->] ->]]". hss. 
 
-    steps_r. destruct (arg ↓) as [args|] eqn : Harg; cycle 1.
-    { sch_yield_l. steps_l. iDestruct "ASM" as "[[% ->] _]"; hss. }
-
-    clear Harg.
+    steps_r. sch_yield_ir.
 
     (* allocate new stack *)
-    steps_r. sch_yield_rr. steps_r.
+    steps_r.
     iApply wsim_mem_alloc; [try prove_inline_cond|try prove_sb_cond|ss|unfold_cris_defs].
     iIntros (stackb) "[↦stack [↦val _]]".
-    steps_r. hss_r. steps_r.
-    sch_yield_rr. steps_r. sch_yield_rr. steps_r.
+    steps_r. hss_r. steps_r. sch_yield_ir.
+    steps_r. sch_yield_ir.
 
     (* initialize stack *)
+    steps_r.
     iApply (wsim_mem_store with "↦stack");
       [try prove_inline_cond|try prove_sb_cond|..|unfold_cris_defs].
-    iIntros "↦stack". steps_r. hss_r. steps_r. sch_yield_rr.
+    iIntros "↦stack". steps_r. hss_r.
+
+    steps_r. sch_yield_ir.
 
     steps_r.
     iApply (wsim_mem_store with "↦val");
       [try prove_inline_cond|try prove_sb_cond|..|unfold_cris_defs].
-    iIntros "↦val". steps_r. hss_r. steps_r. sch_yield_rr. steps_r.
+    iIntros "↦val". steps_r. hss_r.
 
-    sch_yield_l. steps_l. iDestruct "ASM" as "[[% ->] _]"; hss.
+    steps_r. sch_yield_ir.
+    steps_r.
+
+    sch_yield_l.
     iMod (own_alloc (● Excl' [] ⋅ ◯ Excl' [])) as (γs) "[Hs● Hs◯]".
     { apply auth_both_valid_discrete. split; done. }
-    iMod (inv_alloc (syn_stack_inv γs stackb 0%Z 0) _ _ _ stackN with "[-Hs◯ IST]")
+    iMod (inv_alloc (syn_stack_inv N γs stackb 0%Z 0) _ _ _ stackN with "[-Hs◯ IST TID]")
       as "#Hinv"; eauto.
     { apply nclose_subseteq. }
-    { rewrite SLRed_red. iExists (Vint 0), None, []; iFrame; eauto. }
-    force_l ((Vptr (stackb, 0%Z))↑). steps_l. force_l.
-    iFrame "Hs◯"; iSplit; eauto.
+    { rewrite /syn_stack_inv /syn_is_offer SLRed_red. iExists (Vint 0), (Vint 0), []; iFrame; eauto.
+      rewrite SLRed_red //.
+    }
+
+    force_l (Vptr (stackb, 0%Z)). steps_l. forces_l.
+    iFrame "Hs◯ TID"; iSplit; eauto.
     { iSplit; eauto. iExists _; iSplit; eauto. iExists _, _; iSplit; eauto. }
-    steps_l. sch_yield_l. step. iSplit; eauto.
-  Unshelve. all: eauto. all: try exact 0.
-  Qed.
+    steps_l. step. iSplit; eauto.
+  (*SLOW*)Admitted.
 
-  Lemma push_simF : ISim.sim_fun open MA MI init_cond IstFull (Some StackHdr.push).
-  Proof using Hsch.
+  Program Global Instance winv_sep_WP `{!crisG Γ Σ α β τ _S _I} E P :
+    WP (winv (E, E) ∗ P) :=
+    {| WP_space := E; WP_remainder := P |}.
+  Next Obligation. intros; iSplit; iIntros "[$ $]". Qed.
+
+  Lemma push_simF : ISim.sim_fun open StackM StackI init_cond IstFull (Some StackHdr.push).
+  Proof using Hsch Hmsk Hspsch Hsphelp.
     init_simF.
-    steps_l; unfold_lat_img_l.
 
-    (* ill-formed argument *)
-    destruct (classic (∃ blk ofs v, arg = [Vptr (blk, ofs); v]↑)); cycle 1.
-    { admit. }
-    des; subst; hss.
+    steps_l.
+    destruct Hsphelp as [Hfind2 Hfind]; rewrite (Hfind (Helping.run mn) None) //; cycle 1.
+    { rewrite /alist_find eq_rel_dec_correct /=; des_ifs. }
+    clear Hfind Hfind2.
+    rename _q into args, _q3 into stid, _q4 into mtid, _q6 into γs, _q7 into s, _q8 into v.
+    iDestruct "ASM" as "[TID [[% #[%stackb [%stackofs [-> Hinv]]]] _]]"; hss.
 
-    steps_r.
+    (* Register for helping *)
+    steps_r. norm_l.
+    iApply (wsim_helping_run with "IST");
+      [try prove_inline_cond|try prove_sb_cond|unfold_cris_defs|..].
+    clear st_src st_tgt; iIntros (st_src st_tgt req_id) "IST Help".
+
+    (* Coinduction starts here *)
     iApply wsim_reset. iStopProof.
     revert st_src. combine_quant st_tgt.
     eapply wsim_coind.
-    iIntros (g' _ CIH [st_tgt st_src]) "IST /=".
+    iIntros (g' _ CIH [st_tgt st_src]) "[#Hinv [TID [IST Help]]] /=".
     destruct_quant CIH.
 
-    unfold_iter_r; rewrite {1}/StackI._push; steps_r.
-    sch_yield_rr. steps_r. sch_yield_rr. steps_r.
+    unfold_iter_r. rewrite {1}/StackI._push. steps_r.
 
-    (* opening invariant *)
-    sch_yield_l; steps_l. hss.
-    iDestruct "ASM"  as "[[%Heq [[%stackb [%stackofs [-> #Hinv]]] stack]] _]".
-    symmetry in Heq; hss.
-    rename _q1 into γs, _q3 into l.
+    sch_yield_ir. steps_r.
+    sch_yield_ir. steps_r.
 
     (* load *)
     iInv "Hinv" as "Hstack" "close".
-    rewrite SLRed_red.
-    iDestruct "Hstack" as "[%stack_rep [%offer_rep [%l' [Hs [H↦ [Hlist Hoffer]]]]]]".
+    rewrite {1}SLRed_red.
+    iDestruct "Hstack" as "[%stack_rep [%offer_rep [%l [Hs [H↦ [Hlist Hoffer]]]]]]".
 
     iApply (wsim_mem_load with "[H↦]");
       [try prove_inline_cond|try prove_sb_cond|ss|unfold_cris_defs].
@@ -97,31 +167,26 @@ Module StackIM. Section StackIM.
 
     iPoseProof (list_inv_comparable with "Hlist") as "[Hlist [Hval #Hcomp]]".
     iMod ("close" with "[Hs Hlist H↦ Hoffer]") as "_".
-    { rewrite /stack_inv. do 3 (SL_red; iExists _); SL_red; iFrame. }
-    force_l true. steps_l. force_l; iSplitL "stack"; iFrame.
-    { iSplit; eauto. iSplit; eauto. iExists _, _; iFrame "Hinv"; eauto. }
-    steps_l; unfold_lat_img_l. hss.
-    iClear "Hinv". clear dependent l l' γs offer_rep.
+    { rewrite /syn_stack_inv /syn_is_offer.
+      do 3 (SL_red; iExists _); SL_red; iFrame. rewrite SLRed_red //.
+    }
 
     (* alloc new head *)
-    sch_yield_rr. steps_r.
+    sch_yield_ir. steps_r.
     iApply wsim_mem_alloc; [try prove_inline_cond|try prove_sb_cond|ss|unfold_cris_defs].
     iIntros (head_newb) "[Hnewv [Hnewhead _]]". steps_r. hss_r. steps_r.
 
     (* store to new head *)
-    steps_r. sch_yield_rr. steps_r. sch_yield_rr. steps_r.
+    sch_yield_ir. steps_r. sch_yield_ir. steps_r.
     iApply (wsim_mem_store with "Hnewv");
       [try prove_inline_cond|try prove_sb_cond|unfold_cris_defs].
-    iIntros "Hnewv". steps_r. hss_r. steps_r. sch_yield_rr. steps_r.
+    iIntros "Hnewv". steps_r. hss_r. steps_r. sch_yield_ir. steps_r.
     iApply (wsim_mem_store with "Hnewhead");
       [try prove_inline_cond|try prove_sb_cond|unfold_cris_defs].
     iIntros "Hnewhead". steps_r. hss_r. steps_r.
 
     (* try push *)
-    sch_yield_rr. steps_r.
-    steps_l; unfold_lat_img_l. sch_yield_l. steps_l.
-    iDestruct "ASM" as "[[%EQ [#[% [% [-> #Hinv]]] Hl']] _]"; symmetry in EQ; hss.
-    rename _q1 into γs, _q3 into l.
+    sch_yield_ir. steps_r.
     iInv "Hinv" as "Hstack" "close".
     rewrite SLRed_red.
     iDestruct "Hstack" as "[%stack_rep' [%offer_rep' [%l' [Hs [H↦ [Hlist Hoffer]]]]]]".
@@ -135,77 +200,193 @@ Module StackIM. Section StackIM.
     iIntros "H↦ [Hval Hval2]". iClear "Hcomp".
     case_decide; subst.
     { (* success *)
+      clear CIH.
       steps_r. hss_r. steps_r.
-      iCombine "Hs Hl'" gives
+
+      (* atomic update happens here: since it is valid to update stack_contents here (without any
+         helps from other threads), the pusher does its own job *)
+      sch_yield_l. norm_l.
+      iApply (wsim_helping_try_run with "Help IST").
+      clear st_src; iIntros (reqmap st_src) "Help IST".
+      rewrite /StackM.jobCode /=. steps_l.
+      rewrite Helping.trans_take. steps_l. clear l; rename _q into l.
+      rewrite Helping.trans_Assume. steps_l.
+      iCombine "Hs ASM" gives
         %[->%Excl_included%leibniz_equiv _]%auth_both_valid_discrete.
-      iMod (own_update_2 with "Hs Hl'") as "[Hs Hl']".
+      iMod (own_update_2 with "Hs ASM") as "[Hs Hl]".
       { eapply auth_update, option_local_update, (exclusive_local_update _ (Excl _)). done. }
+      rewrite Helping.trans_Guarantee. force_l. iFrame.
+      rewrite Helping.trans_ret. steps_l.
+
+      (* we updated the user-side resource, now proceed *)
       iMod ("close" with "[Hnewv Hnewhead Hoffer Hlist H↦ Hs]") as "_".
       { iExists _, offer_rep', (v :: l'). iFrame. iExists 1%Qp; iSplit; eauto.
         rewrite Z.add_0_l.
         destruct stack_rep, stack_rep'; inv Hcomp; des_ifs.
         simpl_bool; des; do 2 destruct (dec _ _); clarify.
       }
-      force_l false. force_l. force_l. iSplitL "Hl'"; eauto.
-      steps_l.
+      iMod (IstHelp_done with "Help IST") as "[Done IST]".
 
-      sch_yield_rr. steps_r.
+      (* comparison *)
+      sch_yield_ir. steps_r.
       iCombine "Hval" "Hval2" as "Hval".
       iApply (wsim_mem_cmp with "Hval");
         [try prove_inline_cond|try prove_sb_cond|unfold_cris_defs|..]; eauto.
       { iIntros "[[% [% $]] [% [% $]]] !> [$ $] //". }
-      iIntros "_". steps_r. hss_r. steps_r. sch_yield_rr. steps_r. sch_yield_l. step. eauto.
+      iIntros "_". steps_r. hss_r. steps_r.
+
+      (* epilogue *)
+      sch_yield_ir. steps_r. sch_yield_l. steps_l. hss.
+      force_l; iFrame "TID". iSplit; eauto.
+      step.
+      iFrame; done.
     }
 
-    (* failure - make an offer *)
+    (* failure *)
     steps_r. hss_r. steps_r.
     iMod ("close" with "[Hnewv Hnewhead Hoffer Hlist H↦ Hs]") as "_".
     { iExists _, offer_rep', l'. iFrame. }
-    force_l true. force_l. iSplitL "Hl'"; iFrame.
-    { iSplit; eauto. iSplit; eauto. rewrite /is_stack; iExists _, _; iSplit; eauto. }
-    steps_l.
 
-    sch_yield_rr. steps_r.
+    (* comparison - which leads us to offering *)
+    sch_yield_ir. steps_r.
     iCombine "Hval" "Hval2" as "Hval".
     iApply (wsim_mem_cmp with "Hval");
       [try prove_inline_cond|try prove_sb_cond|unfold_cris_defs|..]; eauto.
     { iIntros "[[% [% $]] [% [% $]]] !> [$ $] //". }
-    iIntros "_". steps_r. hss_r. steps_r. sch_yield_rr. steps_r.
+    iIntros "_". steps_r. hss_r. steps_r.
+    sch_yield_ir. steps_r.
     destruct (decide (succ = 0)); subst; cycle 1.
     { exfalso; destruct stack_rep', stack_rep; inv Hcomp; des_ifs. }
 
-    steps_r. sch_yield_rr. steps_r.
+    (* make an offer *)
+    steps_r. sch_yield_ir. steps_r.
     iApply wsim_mem_alloc; [try prove_inline_cond|try prove_sb_cond|ss|unfold_cris_defs].
     iIntros (offerb) "[Hofferv [Hofferst _]]".
     steps_r; hss_r; steps_r.
 
-    sch_yield_rr; steps_r. sch_yield_rr; steps_r.
+    sch_yield_ir. steps_r.
+    sch_yield_ir. steps_r.
     iApply (wsim_mem_store with "[Hofferv]");
       [try prove_inline_cond|try prove_sb_cond|ss|unfold_cris_defs].
     iIntros "Hofferv". steps_r. hss_r. steps_r.
 
-    sch_yield_rr. steps_r.
+    sch_yield_ir. steps_r.
     iApply (wsim_mem_store with "[Hofferst]");
       [try prove_inline_cond|try prove_sb_cond|ss|unfold_cris_defs].
     iIntros "Hofferst". steps_r. hss_r. steps_r.
     rewrite Z.add_0_l.
 
-    sch_yield_rr; steps_r.
+    sch_yield_ir; steps_r.
+    iInv "Hinv" as "Hstack" "close".
+    rewrite {1}SLRed_red. clear dependent l l' stack_rep stack_rep' offer_rep offer_rep'.
+    iDestruct "Hstack" as "[%stack_rep [%offer_rep [%l [Hs [H↦ [Hlist [Hoffer↦ _]]]]]]]".
+    iApply (wsim_mem_store with "Hoffer↦");
+      [try prove_inline_cond|try prove_sb_cond|unfold_cris_defs].
+    iIntros "Hoffer↦". steps_r. hss_r.
+    iMod (own_alloc (Excl ())) as "[%γo OfferTkn]"; ss.
+    iMod (inv_alloc
+      (syn_offer_inv 0 γo (offerb, 0%Z) (stid, mtid, (Vptr (stackb, stackofs), v, γs)))
+      _ _ _ offerN with "[Hofferv Hofferst Help]") as "#Hoinv"; eauto.
+    { apply nclose_subseteq. }
+    { rewrite SLRed_red; iExists _, _; iFrame. done. }
+
+    iMod ("close" with "[Hoffer↦ Hlist H↦ Hs]") as "_".
+    { rewrite SLRed_red. iExists _, (Vptr (offerb, 0%Z)), l. iFrame.
+      rewrite /syn_is_offer /= SLRed_red. iExists γo, _. rewrite inv_red //. }
+    steps_r. sch_yield_ir. steps_r.
+
+    iInv "Hinv" as "Hstack" "close".
+    rewrite {1}SLRed_red. clear dependent l stack_rep offer_rep.
+    iDestruct "Hstack" as "[%stack_rep [%offer_rep [%l [Hs [H↦ [Hlist [Hoffer↦ _]]]]]]]".
+    iApply (wsim_mem_store with "Hoffer↦");
+      [try prove_inline_cond|try prove_sb_cond|unfold_cris_defs].
+    iIntros "Hoffer↦". steps_r. hss_r.
+
+    iMod ("close" with "[Hoffer↦ Hlist H↦ Hs]") as "_".
+    { rewrite SLRed_red. iExists _, _, l. iFrame. rewrite SLRed_red //. }
+    steps_r. sch_yield_ir. steps_r.
+
+    iInv "Hoinv" as "oinv" "close"; rewrite {1}SLRed_red.
+    iDestruct "oinv" as "[%offerst [%rid [offerv↦ [offerst↦ offer]]]] /=".
+    rewrite Z.add_0_l.
+    destruct offerst; try by (iCombine "OfferTkn" "offer" gives %WF).
+    destruct n; try by (iCombine "OfferTkn" "offer" gives %WF).
+    { (* nobody helped*)
+      iApply (wsim_mem_cas _ _ _ _ _ _ _ _ _ _ _ _ _ _ _ _ emp%I with "offerst↦");
+        [try prove_inline_cond|try prove_sb_cond|unfold_cris_defs|..]; eauto.
+      des_ifs_safe. iIntros "Hofferst _". steps_r. hss_r. steps_r.
+
+      iMod ("close" with "[offerv↦ Hofferst OfferTkn]") as "_".
+      { rewrite SLRed_red. iExists _, _. iFrame. done. }
+
+      steps_r. sch_yield_ir. steps_r.
+      iAssert (emp)%I as "E"; first done.
+      iApply (wsim_mem_cmp with "E");
+        [try prove_inline_cond|try prove_sb_cond|unfold_cris_defs|..]; eauto.
+      iIntros "_". steps_r. hss_r. steps_r.
+
+      by_coind CIH. iFrame.
+      (* TODO : make request id explicit in the invariant *)
+      admit.
+    }
+    (* Helped! *)
+  (*SLOW*)Admitted.
+
+  Lemma pop_simF : ISim.sim_fun open StackM StackI init_cond IstFull (Some StackHdr.pop).
+  Proof.
+    init_simF.
+    steps_l. iDestruct "ASM" as "[TID [[% #[%stackb [%stackofs [-> Hinv]]]] _]]". hss.
+    rename _q3 into stid, _q4 into mtid, _q6 into γs.
+    steps_r.
+
+    (* Coinduction starts here *)
+    iApply wsim_reset. iStopProof.
+    revert st_src. combine_quant st_tgt.
+    eapply wsim_coind.
+    iIntros (g' _ CIH [st_tgt st_src]) "[#Hinv [TID [IST Help]]] /=".
+    destruct_quant CIH.
+
+    unfold_iter_r. rewrite {1}/StackI._pop. steps_r.
+    sch_yield_ir. steps_r. sch_yield_ir. steps_r.
+
+    (* Stack load *)
+    iInv "Hinv" as "Hstack" "close".
+    rewrite SLRed_red.
+    iDestruct "Hstack" as "[%stack_rep [%offer_rep [%l [Hs [H↦ [Hlist Hoffer]]]]]]".
+
+    iApply (wsim_mem_load with "[H↦]");
+      [try prove_inline_cond|try prove_sb_cond|ss|unfold_cris_defs].
+    iIntros "H↦". steps_r. hss_r. steps_r.
+
+    destruct (decide (stack_rep = Vint 0%Z)); subst.
+    { (* Empty stack - terminate *)
+      sch_yield_l. steps_l.
+      destruct Hsphelp as [Hfind2 Hfind]; rewrite (Hfind (Helping.help mn) None) //; cycle 1.
+      { rewrite /alist_find eq_rel_dec_correct /=; des_ifs; destruct (dec _ _); ss. }
+      clear Hfind Hfind2.
+
+      iDestruct "IST" as "[% [% [-> [Help● IST]]]]".
+      inline_l. steps_l. force_l (fresh (dom reqmap)). steps_l.
+      rewrite /HoareCall_prologue; unseal "Help".
+      unfold_sp_exact sp (SchHdr.yield); ss.
+      force_l (stid, mtid). steps_l.
+      force_l (()↑).
+      iDestruct "Help●" as "[Help● Help●2]".
+      force_l.
+      admit. 
+    }
+    iPoseProof (list_inv_comparable with "Hlist") as "[Hlist [Hval #Hcomp]]".
+    admit.
   Admitted.
 
   (* Construct ISim.t for summing up each simulation proofs *)
-  Lemma sim : ISim.t open MA MI init_cond IstFull.
-  Proof.
-    init_sim.
-    { split; et. }
-    { apply new_stack_simF. }
-    { apply push_simF. }
-  Qed.
+  Lemma sim : ISim.t open StackM StackI init_cond IstFull.
+  Admitted.
 
   (* ctxr works as a unit in compositions of module simulations *)
-  Lemma ctxr :
+  (* Lemma ctxr :
     ctx_refines
       (StackM.t N ★ MemA.t, emp%I)
       (StackI.t ★ MemA.t, emp%I).
-  Proof. eapply main_adequacy, sim; eauto. Qed.
+  Proof. eapply main_adequacy, sim; eauto. Qed. *)
 End StackIM. End StackIM.
